@prefix csdls: <https://vocabs.sshopencloud.eu/vocabularies/csd-linguistic-subjects/> .
@prefix csdtt: <https://vocabs.sshopencloud.eu/vocabularies/csd-tool-tasks/> .
@prefix dc: <http://purl.org/dc/elements/1.1/> .
@prefix dct: <http://purl.org/dc/terms/> .
@prefix iso639-3: <https://iso639-3.sil.org/code/> .
@prefix owl: <http://www.w3.org/2002/07/owl#> .
@prefix rdfs: <http://www.w3.org/2000/01/rdf-schema#> .
@prefix skos: <http://www.w3.org/2004/02/skos/core#> .
@prefix tadirah: <https://vocabs.dariah.eu/tadirah/> .
@prefix xsd: <http://www.w3.org/2001/XMLSchema#> .

<http://hdl.handle.net/11459/CCR_C-2627_5bd2c71a-8e43-a61d-0897-165b6068cb26> skos:exactMatch csdtt:0029 .

<http://hdl.handle.net/11459/CCR_C-3932_4238a16a-1838-107c-0345-e31ad6d0f6b0> skos:exactMatch csdtt:0039 .

tadirah:analyzing skos:exactMatch csdtt:0004 .

tadirah:authorshipAttribution skos:exactMatch csdtt:0008 .

tadirah:browsing skos:narrower csdtt:0017 .

tadirah:clusterAnalysis skos:closeMatch csdtt:0011 .

tadirah:dataCleansing skos:narrower csdtt:0018 .

tadirah:discovering skos:narrower tadirah:informationRetrieval .

tadirah:enriching skos:narrower csdtt:0006 .

tadirah:georeferencing skos:exactMatch csdtt:0121 .

tadirah:imaging skos:closeMatch csdtt:0111 .

tadirah:namedEntityRecognition skos:closeMatch csdtt:0057 .

tadirah:posTagging skos:exactMatch csdtt:0068 .

tadirah:relationalAnalysis skos:narrower tadirah:principalComponentAnalysis .

tadirah:searching skos:closeMatch csdtt:0078 .

tadirah:sentimentAnalysis skos:closeMatch csdtt:0084 .

tadirah:stylisticAnalysis skos:narrower tadirah:principalComponentAnalysis .

tadirah:topicModeling skos:closeMatch csdtt:0103 .

csdls:0020 skos:related csdtt:0052 .

csdls:0021 skos:related csdtt:0050 .

csdls:0024 skos:related csdtt:0064 .

csdls:0027 skos:related csdtt:0070 .

csdls:0033 skos:related csdtt:0081 .

csdls:0035 skos:related csdtt:0086 .

csdls:0038 skos:related csdtt:0095 .

csdls:0044 skos:related csdtt:0096 .

csdls:0046 skos:related csdtt:0058 .

csdls:0047 skos:related csdtt:0056 .

csdtt:0000 skos:inScheme csdtt: ;
    skos:topConceptOf csdtt: .

csdtt:0002 a skos:Concept ;
    skos:broader csdtt:0064 ;
    skos:definition "A tool's ability to expand an abbreviation to its full form."@en ;
    skos:inScheme csdtt: ;
    skos:prefLabel "abbreviation expansion"@en .

csdtt:0003 a skos:Concept ;
    skos:broader csdtt:0122 ;
    skos:definition "The identification of the corresponding elements or sequences of elements (e.g., sentences, words) in a sequence of elements."@en ;
    skos:inScheme csdtt: ;
    skos:prefLabel "alignment"@en .

csdtt:0005 a skos:Concept ;
    skos:broader csdtt:0081 ;
    skos:definition "mining the historical development of concepts and the vocabulary with which they are expressed"@en ;
    skos:inScheme csdtt: ;
    skos:prefLabel "analysis of concepts across time"@en .

csdtt:0009 a skos:Concept ;
    skos:broader csdtt:0017 ;
    skos:definition "quick examination of the relevance of a number of objects which may or may not lead to a closer examination or acquisition/selection of (some of) these objects (source: Wikipedia)"@en ;
    skos:inScheme csdtt: ;
    skos:prefLabel "browsing"@en .

csdtt:0012 a skos:Concept ;
    skos:broader csdtt:0050 ;
    skos:definition "splitting a word into a sequence of words"@en ;
    skos:inScheme csdtt: ;
    skos:prefLabel "compound splitting"@en .

csdtt:0013 a skos:Concept ;
    skos:broader csdtt:0066 ;
    skos:definition "Constituency-based parsing is a type of parsing in which a sentence is split up into constituents or phrases (such as VP or NP)."@en ;
    skos:inScheme csdtt: ;
    skos:prefLabel "constituency-based parsing"@en .

csdtt:0014 a skos:Concept ;
    skos:broader csdtt:0056 ;
    skos:definition "tool to find linguistic objects (words, sentences, etc.) that co-occur with a given linguistic object"@en ;
    skos:inScheme csdtt: ;
    skos:prefLabel "co-occurence addition"@en .

csdtt:0015 a skos:Concept ;
    skos:broader csdtt:0028 ;
    skos:definition "enriching a text with co-reference markings"@en ;
    skos:inScheme csdtt: ;
    skos:prefLabel "co-reference assignment"@en .

csdtt:0016 a skos:Concept ;
    skos:broader csdtt:0028 ;
    skos:definition "Co-reference resolution is the task of finding all expressions that refer to the same entity in a text."@en ;
    skos:inScheme csdtt: ;
    skos:prefLabel "co-reference resolution"@en .

csdtt:0022 a skos:Concept ;
    skos:broader csdtt:0020 ;
    skos:definition "A corpus workbench is a collection of tools for managing and processing corpora."@en ;
    skos:inScheme csdtt: ;
    skos:prefLabel "corpus workbench"@en .

csdtt:0023 a skos:Concept ;
    skos:broader csdtt:0066 ;
    skos:definition "Dependency parsing is a type of parsing in which asymmetric, binary relations are assigned between lexical items. One part in such a relation is called the head, the other the dependent."@en ;
    skos:inScheme csdtt: ;
    skos:prefLabel "dependency parsing"@en .

csdtt:0024 a skos:Concept ;
    skos:broader csdtt:0086 ;
    skos:definition "Dialectometry is the (quantitative) study of the regional distribution of dialects."@en ;
    skos:inScheme csdtt: ;
    skos:prefLabel "dialectometry"@en .

csdtt:0025 a skos:Concept ;
    skos:broader csdtt:0028 ;
    skos:definition "Dialogue management refers to the part of a dialogue system that is responsible for controlling the architecture and structure of the dialogue."@en ;
    skos:inScheme csdtt: ;
    skos:prefLabel "dialogue management"@en .

csdtt:0026 a skos:Concept ;
    rdfs:isDefinedBy <https://en.wiktionary.org/wiki/diarization> ;
    skos:broader csdtt:0112 ;
    skos:definition "In voice recognition, the process of partitioning an input audio stream into homogeneous segments according to the speaker identity, so as to identify different speakers' turns in a conversation"@en ;
    skos:inScheme csdtt: ;
    skos:prefLabel "diarization"@en .

csdtt:0027 a skos:Concept ;
    skos:broader csdtt:0114 ;
    skos:definition "text search in a dictionary (considered as  a sequence of characters)"@en ;
    skos:inScheme csdtt: ;
    skos:prefLabel "dictionary searching"@en .

csdtt:0030 a skos:Concept ;
    rdfs:isDefinedBy <https://en.wikipedia.org/wiki/Editing> ;
    skos:definition "the process of selecting and preparing written, photographic, visual, audible, or cinematic material used by a person or an entity to convey a message or information. The editing process can involve correction, condensation, organisation, and many other modifications performed with an intention of producing a correct, consistent, accurate and complete piece of work."@en ;
    skos:inScheme csdtt: ;
    skos:prefLabel "editing"@en ;
    skos:topConceptOf csdtt: .

csdtt:0031 a skos:Concept ;
    skos:definition "assessing the usefulness of a resource for a particular task"@en ;
    skos:inScheme csdtt: ;
    skos:prefLabel "evaluation"@en ;
    skos:topConceptOf csdtt: .

csdtt:0032 a skos:Concept ;
    skos:broader csdtt:0004 ;
    skos:definition "selecting elements to exclude them"@en ;
    skos:inScheme csdtt: ;
    skos:prefLabel "filtering"@en .

csdtt:0033 a skos:Concept ;
    skos:broader csdtt:0020 ;
    skos:definition "changing data from one format to another"@en ;
    skos:inScheme csdtt: ;
    skos:prefLabel "format conversion"@en .

csdtt:0034 a skos:Concept ;
    <http://www.w3.org/2000/01/rdf-schema#seeAlso:> <https://en.wikipedia.org/wiki/Geographic_coordinate_system> ;
    skos:broader csdtt:0121 ;
    skos:definition "assigning the coordinates of a geographic coordinate system  to an object"@en ;
    skos:inScheme csdtt: ;
    skos:prefLabel "geographical coordinate assignment"@en .

csdtt:0035 a skos:Concept ;
    skos:broader csdtt:0066 ;
    skos:definition "connecting words or word groups and name the grammatical relation between them."@en ;
    skos:inScheme csdtt: ;
    skos:prefLabel "grammatical relation assignment"@en .

csdtt:0036 a skos:Concept ;
    rdfs:seeAlso <https://en.wikipedia.org/wiki/Associative_array> ;
    skos:broader csdtt:0125 ;
    skos:definition "assigning indexes, i.e. keys in an associative array, to objects"@en ;
    skos:inScheme csdtt: ;
    skos:prefLabel "indexing"@en .

csdtt:0037 a skos:Concept ;
    skos:broader csdtt:0020 ;
    skos:definition "extracting important words in a text that are useful to indicate the text's meaning."@en ;
    skos:inScheme csdtt: ;
    skos:prefLabel "keyword extraction"@en .

csdtt:0038 a skos:Concept ;
    rdfs:seeAlso <https://en.wikipedia.org/wiki/Knowledge_representation_and_reasoning> ;
    skos:broader csdtt:0123 ;
    skos:definition "creating a representation for  information about the world in a form that a computer system can use to reason and/or solve complex tasks"@en ;
    skos:inScheme csdtt: ;
    skos:prefLabel "knowledge representation"@en .

csdtt:0040 a skos:Concept ;
    skos:broader csdtt:0050 ;
    skos:definition "assigning a lemma to an inflected word form"@en ;
    skos:inScheme csdtt: ;
    skos:prefLabel "lemmatisation"@en .

csdtt:0041 a skos:Concept ;
    rdfs:seeAlso <https://en.wikipedia.org/wiki/Lexicon> ;
    skos:broader csdtt:0114 ;
    skos:definition "creation of a lexicon"@en ;
    skos:inScheme csdtt: ;
    skos:prefLabel "lexicon creation"@en .

csdtt:0046 a skos:Concept ;
    skos:broader csdtt:0053 ;
    skos:definition "the automatic translation of text or speech from one natural language to another."@en ;
    skos:inScheme csdtt: ;
    skos:prefLabel "machine translation"@en .

csdtt:0047 a skos:Concept ;
    skos:altLabel "metadating"@en ;
    skos:broader csdtt:0124 ;
    skos:definition "the creation of metadata"@en ;
    skos:inScheme csdtt: ;
    skos:prefLabel "metadata creation"@en .

csdtt:0049 a skos:Concept ;
    skos:broader csdtt:0050 ;
    skos:definition "Morphological analysis is the process of analysing the internal structure of a word, i.e. recognizing the morphemes that together constitute a word."@en ;
    skos:inScheme csdtt: ;
    skos:prefLabel "morphological analysis"@en .

csdtt:0051 a skos:Concept ;
    skos:broader csdtt:0052 ;
    skos:definition "assigning morpho-syntactic properties to occurrences of word forms in a text"@en ;
    skos:inScheme csdtt: ;
    skos:prefLabel "morphosyntactic tagging"@en .

csdtt:0054 a skos:Concept ;
    skos:broader csdtt:0056 ;
    skos:definition "locating the position of a multiword expression in a text"@en ;
    skos:inScheme csdtt: ;
    skos:prefLabel "multiword expression identification"@en .

csdtt:0055 a skos:Concept ;
    skos:broader csdtt:0056 ;
    skos:definition "A tool's ability to recognize multi-word expressions or units (MWUs). An MWU is an expression formed by two or more words that has properties that cannot be derived from its component words or the way they are combined by regular rules."@en ;
    skos:inScheme csdtt: ;
    skos:prefLabel "multiword unit identification"@en .

csdtt:0059 a skos:Concept ;
    rdfs:isDefinedBy <https://en.wikipedia.org/wiki/Digital_image_processing> ;
    skos:broader csdtt:0127 ;
    skos:definition "Natural language generation (NLG) is a software process that produces natural language output."@en ;
    skos:inScheme csdtt: ;
    skos:prefLabel "natural language generation"@en .

csdtt:0060 a skos:Concept ;
    skos:broader csdtt:0128 ;
    skos:definition "Natural language understanding is a software process that deals with comprehension of natural language input"@en ;
    skos:inScheme csdtt: ;
    skos:prefLabel "natural language understanding"@en .

csdtt:0061 a skos:Concept ;
    skos:broader csdtt:0064 ;
    skos:definition "Number expansion is the process of converting numbers in a text to their full written-out forms."@en ;
    skos:inScheme csdtt: ;
    skos:prefLabel "number expansion"@en .

csdtt:0065 a skos:Concept ;
    skos:definition "tool task not covered by any other tool task"@en ;
    skos:inScheme csdtt: ;
    skos:prefLabel "other"@en ;
    skos:topConceptOf csdtt: .

csdtt:0067 a skos:Concept ;
    skos:broader csdtt:0052 ;
    skos:definition "creating part of speech codes for a word"@en ;
    skos:inScheme csdtt: ;
    skos:prefLabel "part of speech generation"@en .

csdtt:0069 a skos:Concept ;
    skos:broader csdtt:0070 ;
    skos:definition "Phonetic annotation is the process of adding information about speech sounds to a text in written form, usually using a phonetic alphabet such as IPA."@en ;
    skos:inScheme csdtt: ;
    skos:prefLabel "phonetic annotation"@en .

csdtt:0071 skos:inScheme csdtt: ;
    skos:topConceptOf csdtt: .

csdtt:0072 a skos:Concept ;
    skos:broader csdtt:0113 ;
    skos:definition "software to obtain characteristics of an object"@en ;
    skos:inScheme csdtt: ;
    skos:prefLabel "profiling"@en .

csdtt:0073 a skos:Concept ;
    dct:isReplacedBy csdtt:0078 ;
    owl:deprecated true ;
    skos:Label "querying"@en ;
    skos:broader csdtt:0077 ;
    skos:changeNote "querying is now an altLabel for searching" ;
    skos:definition "defining a search request by means of a query"@en ;
    skos:inScheme csdtt: ;
    skos:prefLabel "querying"@en .

csdtt:0075 a skos:Concept ;
    rdfs:seeAlso <https://en.wikipedia.org/wiki/Readability> ;
    skos:broader csdtt:0113 ;
    skos:definition "a variety of software programs to determine the readability of a written text"@en ;
    skos:inScheme csdtt: ;
    skos:prefLabel "readability analysis"@en .

csdtt:0076 a skos:Concept ;
    skos:broader csdtt:0066 ;
    skos:definition "Relation extraction is the process of detecting and classifying relationships within a text."@en ;
    skos:inScheme csdtt: ;
    skos:prefLabel "relation extraction"@en .

csdtt:0079 a skos:Concept ;
    skos:broader csdtt:0081 ;
    skos:definition "a process to add entries to a semantic registry and mapping these entries to labels (terms)"@en ;
    skos:inScheme csdtt: ;
    skos:prefLabel "semantic registry and mapping"@en .

csdtt:0080 a skos:Concept ;
    skos:broader csdtt:0081 ;
    skos:definition "Semantic role labelling is the process of automatically finding the semantic roles (such as agent or patient) for each predicate in a sentence."@en ;
    skos:inScheme csdtt: ;
    skos:prefLabel "semantic role labeling"@en .

csdtt:0082 a skos:Concept ;
    skos:broader csdtt:0064 ;
    skos:definition "selection of sentences from a text corpus"@en ;
    skos:inScheme csdtt: ;
    skos:prefLabel "sentence selection"@en .

csdtt:0083 a skos:Concept ;
    skos:broader csdtt:0064 ;
    skos:definition "turning a sequence of characters or words into a sequence of sentences"@en ;
    skos:inScheme csdtt: ;
    skos:prefLabel "sentence splitting"@en .

csdtt:0087 a skos:Concept ;
    rdfs:isDefinedBy <https://en.wikipedia.org/wiki/Speech_recognition> ;
    skos:broader csdtt:0112 ;
    skos:definition "software to recognise spoken natural language and convert it to  text or actions"@en ;
    skos:inScheme csdtt: ;
    skos:prefLabel "speech recognition"@en .

csdtt:0088 a skos:Concept ;
    rdfs:isDefinedBy <https://en.wikipedia.org/wiki/Speech_segmentation> ;
    skos:broader csdtt:0112 ;
    skos:definition "software to identify the boundaries between words, syllables, or phonemes in spoken natural languages"@en ;
    skos:inScheme csdtt: ;
    skos:prefLabel "speech segmentation"@en .

csdtt:0090 a skos:Concept ;
    skos:broader csdtt:0064 ;
    skos:definition "Spell checking is the process of recognizing words in a document that may not be spelled correctly."@en ;
    skos:inScheme csdtt: ;
    skos:prefLabel "spell checking"@en .

csdtt:0091 a skos:Concept ;
    skos:broader csdtt:0050 ;
    skos:definition "Stemming is the process of converting inflected words to their word stem, base or root form."@en ;
    skos:inScheme csdtt: ;
    skos:prefLabel "stemming"@en .

csdtt:0092 a skos:Concept ;
    rdfs:seeAlso <https://en.wikipedia.org/wiki/Forensic_linguistics#Forensic_stylistics> ;
    skos:broader csdtt:0113 ;
    skos:definition "software to determine stylistic properties of a natural language text"@en ;
    skos:inScheme csdtt: ;
    skos:prefLabel "stylistic analysis"@en .

csdtt:0093 a skos:Concept ;
    skos:broader csdtt:0100 ;
    skos:definition "Summarisation is the process of reducing a text document to a summary that retains the most important points of the original document."@en ;
    skos:inScheme csdtt: ;
    skos:prefLabel "summarisation"@en .

csdtt:0094 a skos:Concept ;
    skos:broader csdtt:0066 ;
    skos:definition "analysis in terms of syntactic concepts"@en ;
    skos:inScheme csdtt: ;
    skos:prefLabel "syntactic analysis"@en .

csdtt:0098 a skos:Concept ;
    skos:broader csdtt:0100 ;
    skos:definition "conversion of a text"@en ;
    skos:inScheme csdtt: ;
    skos:prefLabel "text conversion"@en .

csdtt:0099 a skos:Concept ;
    skos:broader csdtt:0100 ;
    skos:definition "Text mining refers to the process of deriving high-quality information from text. Typical text mining tasks include text categorization, concept/entity extraction, sentiment analysis and document summarization."@en ;
    skos:inScheme csdtt: ;
    skos:prefLabel "text mining"@en .

csdtt:0101 a skos:Concept ;
    rdfs:seeAlso <https://en.wikipedia.org/wiki/Speech_synthesis> ;
    skos:broader csdtt:0112 ;
    skos:definition "software to convert natural language text into speech"@en ;
    skos:inScheme csdtt: ;
    skos:prefLabel "text to speech"@en .

csdtt:0102 a skos:Concept ;
    skos:broader csdtt:0064 ;
    skos:definition "turning a sequence of characters (a text) into a sequence of occurrences of inflected word forms and interpunction symbols (often called 'tokens')"@en ;
    skos:inScheme csdtt: ;
    skos:prefLabel "tokenisation"@en .

csdtt:0104 a skos:Concept ;
    rdfs:seeAlso <https://en.wikipedia.org/wiki/Topic_model> ;
    skos:broader csdtt:0113 ;
    skos:definition "software to discover one or more topics in a text"@en ;
    skos:inScheme csdtt: ;
    skos:prefLabel "topic recognition"@en .

csdtt:0106 a skos:Concept ;
    skos:broader csdtt:0007 ;
    skos:definition "converting an audio or video file into a different sample rate"@en ;
    skos:inScheme csdtt: ;
    skos:prefLabel "up-down sampling"@en .

csdtt:0107 a skos:Concept ;
    skos:broader csdtt:0007 ;
    skos:definition "recognising objects and actions in a video"@en ;
    skos:inScheme csdtt: ;
    skos:prefLabel "video recognition"@en .

csdtt:0108 a skos:Concept ;
    rdfs:isDefinedBy <https://en.wikipedia.org/wiki/Data_and_information_visualization> ;
    skos:broader csdtt:0126 ;
    skos:definition "software to create visual representations of complex data and information"@en ;
    skos:inScheme csdtt: ;
    skos:prefLabel "visualisation"@en .

csdtt:0109 a skos:Concept ;
    skos:broader csdtt:0050 ;
    skos:definition "Word segmentation is the process of extracting words from continuous speech."@en ;
    skos:inScheme csdtt: ;
    skos:prefLabel "word segmentation"@en .

csdtt:0110 a skos:Concept ;
    skos:broader csdtt:0081 ;
    skos:definition "Word sense disambiguation is the process of identifying the right sense or meaning of a word when it has multiple meanings by making use of the context in which the word is used"@en ;
    skos:inScheme csdtt: ;
    skos:prefLabel "word sense disambiguation"@en .

csdtt:0119 a skos:Concept ;
    skos:broader csdtt:0113 ;
    skos:definition "determine the identity of the author of a text"@en ;
    skos:inScheme csdtt: ;
    skos:prefLabel "authorship identification"@en .

csdtt:0120 a skos:Concept ;
    rdfs:isDefinedBy <https://en.wikipedia.org/wiki/Author_profiling> ;
    skos:broader csdtt:0113 ;
    skos:definition "determine characteristics of the author of a text"@en ;
    skos:inScheme csdtt: ;
    skos:prefLabel "authorship profiling"@en .

<http://hdl.handle.net/11459/CCR_C-2591_f769d93b-c007-d2c9-aff2-99e9177e5764> skos:related csdtt:0105 ;
    skos:relatedMatch csdtt:0105 .

<http://hdl.handle.net/11459/CCR_C-4428_10017d9a-0387-0a2b-1fbb-515a47bf1ed9> skos:related csdtt:0074 ;
    skos:relatedMatch csdtt:0074 .

tadirah:annotating skos:exactMatch csdtt:0006 ;
    skos:narrower csdtt:0057 .

tadirah:capturing skos:narrower csdtt:0089,
        csdtt:0111 .

tadirah:collocationAnalysis a <http://www.w3.org/2002/07/owl#NamedIndividual:Concept>,
        skos:concept ;
    skos:broader tadirah:structuralAnalysis,
        csdtt:0056 ;
    skos:inScheme tadirah: ;
    skos:note "analysis of recurrent co-occurrences of two or more words in language."@en ;
    skos:prefLabel "Collocation Analysis"@en .

tadirah:concordance a owl:NamedIndividual,
        skos:concept ;
    skos:broader tadirah:structuralAnalysis,
        csdtt:0020 ;
    skos:definition "list of words or terms in a published book (Wikidata contributors, \"Q839018,\" Wikidata, https://www.wikidata.org/w/index.php?title=Q839018&oldid=1228232199 (accessed July 30, 2020)."@en ;
    skos:inScheme tadirah: ;
    skos:prefLabel "Concordance"@en .

tadirah:informationRetrieval a owl:NamedIndividual,
        skos:concept ;
    skos:broader tadirah:contentAnalysis,
        tadirah:discovering ;
    skos:definition "activity of obtaining information resources relevant to an information need from a collection of information resources (Wikidata contributors, \"Q816826,\" Wikidata, https://www.wikidata.org/w/index.php?title=Q816826&oldid=1228359828 (accessed July 30, 2020)."@en ;
    skos:inScheme tadirah: ;
    skos:prefLabel "Information Retrieval"@en .

tadirah:principalComponentAnalysis a owl:NamedIndividual,
        skos:concept ;
    skos:broader tadirah:relationalAnalysis,
        tadirah:stylisticAnalysis ;
    skos:definition "conversion of a set of observations of possibly correlated variables into a set of values of linearly uncorrelated variables called principal components (Wikidata contributors, \"Q2873,\" Wikidata, https://www.wikidata.org/w/index.php?title=Q2873&oldid=1237203694 (accessed July 30, 2020)."@en ;
    skos:inScheme tadirah: ;
    skos:prefLabel "Principal Component Analysis"@en .

csdtt:0008 a skos:Concept ;
    skos:broader csdtt:0113 ;
    skos:definition "determine whether the author of a  text is a given person"@en ;
    skos:exactMatch tadirah:authorshipAttribution ;
    skos:inScheme csdtt: ;
    skos:prefLabel "authorship attribution"@en .

csdtt:0010 a skos:Concept ;
    skos:broader csdtt:0066,
        csdtt:0085 ;
    skos:definition "assigning partial syntactic structures"@en ;
    skos:inScheme csdtt: ;
    skos:prefLabel "chunking"@en .

csdtt:0011 a skos:Concept ;
    skos:broader csdtt:0004 ;
    skos:closeMatch tadirah:clusterAnalysis ;
    skos:definition "grouping sets of objects in such a way that objects in the same group are more similar to each other than to those in other groups."@en ;
    skos:inScheme csdtt: ;
    skos:prefLabel "clustering"@en .

csdtt:0018 a skos:Concept ;
    skos:broader tadirah:dataCleansing,
        csdtt:0020 ;
    skos:definition "Corpus clean-up is the process of removing noise (for instance markup) or unwanted elements from a corpus."@en ;
    skos:inScheme csdtt: ;
    skos:prefLabel "corpus clean-up"@en .

csdtt:0021 a skos:Concept ;
    skos:broader csdtt:0019,
        csdtt:0077 ;
    skos:definition "searching in  a corpus via a query"@en ;
    skos:inScheme csdtt: ;
    skos:prefLabel "corpus searching"@en .

csdtt:0029 a skos:Concept ;
    skos:broader csdtt:0028 ;
    skos:definition "analysis in terms of discourse concepts"@en ;
    skos:exactMatch <http://hdl.handle.net/11459/CCR_C-2627_5bd2c71a-8e43-a61d-0897-165b6068cb26> ;
    skos:inScheme csdtt: ;
    skos:prefLabel "discourse analysis"@en .

csdtt:0039 a skos:Concept ;
    rdfs:seeAlso <https://en.wikipedia.org/wiki/Language_identification> ;
    skos:broader csdtt:0113 ;
    skos:definition "determining for a piece of  textual or speech content which language it is in"@en ;
    skos:exactMatch <http://hdl.handle.net/11459/CCR_C-3932_4238a16a-1838-107c-0345-e31ad6d0f6b0> ;
    skos:inScheme csdtt: ;
    skos:prefLabel "language identification"@en .

csdtt:0042 a skos:Concept ;
    skos:broader csdtt:0077,
        csdtt:0114 ;
    skos:definition "checking for the presence of a key in a lexicon and returning the entry associated with the key"@en ;
    skos:inScheme csdtt: ;
    skos:prefLabel "lexicon lookup"@en .

csdtt:0043 a skos:Concept ;
    skos:broader csdtt:0077,
        csdtt:0114 ;
    skos:definition "text search in a lexicon"@en ;
    skos:inScheme csdtt: ;
    skos:prefLabel "lexicon searching"@en .

csdtt:0062 a skos:Concept ;
    skos:broader csdtt:0097,
        csdtt:0111 ;
    skos:definition "the electronic or mechanical conversion of images of typed, handwritten or printed text into machine-encoded text"@en ;
    skos:inScheme csdtt: ;
    skos:prefLabel "optical character recognition"@en .

csdtt:0063 a skos:Concept ;
    skos:broader csdtt:0064,
        csdtt:0066 ;
    skos:definition "normalises written text by replacing misspellings, OCR-errors, etc."@en ;
    skos:inScheme csdtt: ;
    skos:prefLabel "orthographic normalisation"@en .

csdtt:0085 a skos:Concept ;
    skos:broader csdtt:0095 ;
    skos:definition "Shallow parsing is a form of sentence analysis in which constituents or phrases are recognised, but their internal structure is not further specified."@en ;
    skos:inScheme csdtt: ;
    skos:narrower csdtt:0010 ;
    skos:prefLabel "shallow parsing"@en .

csdtt:0089 a skos:Concept ;
    rdfs:isDefinedBy <https://en.wikipedia.org/wiki/Transcription_(linguistics)> ;
    skos:broader tadirah:capturing,
        csdtt:0112 ;
    skos:definition "software to convert spoken language into text"@en ;
    skos:inScheme csdtt: ;
    skos:prefLabel "speech transcription"@en .

csdtt:0097 a skos:Concept ;
    skos:broader csdtt:0096 ;
    skos:definition "Terminology extraction refers to the automatic extraction of relevant terms from a text. What is relevant depends on the specific task, for example relevant terms could be keywords or words that are difficult to comprehend."@en ;
    skos:inScheme csdtt: ;
    skos:narrower csdtt:0062 ;
    skos:prefLabel "terminology extraction"@en .

csdtt:0122 a skos:Concept ;
    skos:definition "processing of strings (sequences of characters)"@en ;
    skos:inScheme csdtt: ;
    skos:narrower csdtt:0003 ;
    skos:prefLabel "string processing"@en ;
    skos:topConceptOf csdtt: .

csdtt:0124 a skos:Concept ;
    skos:definition "processing data that provides information about other data"@en ;
    skos:inScheme csdtt: ;
    skos:narrower csdtt:0047 ;
    skos:prefLabel "metadata processing"@en ;
    skos:topConceptOf csdtt: .

csdtt:0125 a skos:Concept ;
    skos:definition "processing organized collections of data"@en ;
    skos:inScheme csdtt: ;
    skos:narrower csdtt:0036 ;
    skos:prefLabel "database processing"@en ;
    skos:topConceptOf csdtt: .

csdtt:0126 a skos:Concept ;
    skos:definition "a mode of communication that conveys information from a speaker to an audience"@en ;
    skos:inScheme csdtt: ;
    skos:narrower csdtt:0108 ;
    skos:prefLabel "presentation"@en ;
    skos:topConceptOf csdtt: .

csdtt:0127 a skos:Concept ;
    skos:definition "the process of creating natural language expressions"@en ;
    skos:inScheme csdtt: ;
    skos:narrower csdtt:0059 ;
    skos:prefLabel "generation"@en ;
    skos:topConceptOf csdtt: .

csdtt:0128 a skos:Concept ;
    skos:definition "the process of interpreting natural language expressions"@en ;
    skos:inScheme csdtt: ;
    skos:narrower csdtt:0060 ;
    skos:prefLabel "understanding"@en ;
    skos:topConceptOf csdtt: .

tadirah:structuralAnalysis skos:narrower tadirah:collocationAnalysis,
        tadirah:concordance,
        csdtt:0068 .

csdtt:0007 a skos:Concept ;
    skos:definition "processing  audio and video files"@en ;
    skos:inScheme csdtt: ;
    skos:narrower csdtt:0106,
        csdtt:0107 ;
    skos:prefLabel "audio-visual processing"@en ;
    skos:topConceptOf csdtt: .

csdtt:0017 a skos:Concept ;
    skos:broader tadirah:browsing,
        csdtt:0019 ;
    skos:definition "looking through the contents of a resource"@en ;
    skos:inScheme csdtt: ;
    skos:narrower csdtt:0009 ;
    skos:prefLabel "corpus browsing"@en .

csdtt:0019 a skos:Concept ;
    skos:definition "investigating the composition and contents of a corpus"@en ;
    skos:inScheme csdtt: ;
    skos:narrower csdtt:0017,
        csdtt:0021 ;
    skos:prefLabel "corpus exploration"@en ;
    skos:topConceptOf csdtt: .

csdtt:0053 a skos:Concept ;
    skos:broader csdtt:0044,
        csdtt:0045 ;
    skos:definition "processing involving multiple languages"@en ;
    skos:inScheme csdtt: ;
    skos:narrower csdtt:0046 ;
    skos:prefLabel "multilingual processing"@en .

csdtt:0068 a skos:Concept ;
    skos:broader tadirah:structuralAnalysis,
        csdtt:0052 ;
    skos:definition "Part-of-speech (POS) tagging is the process of assigning a syntactic word category (POS) label to each word in a text."@en ;
    skos:exactMatch tadirah:posTagging ;
    skos:inScheme csdtt: ;
    skos:prefLabel "part of speech tagging"@en .

csdtt:0074 a skos:Concept ;
    skos:broader csdtt:0123 ;
    skos:definition "software to provide an answer to a question posed"@en ;
    skos:inScheme csdtt: ;
    skos:prefLabel "question answering"@en ;
    skos:related <http://hdl.handle.net/11459/CCR_C-4428_10017d9a-0387-0a2b-1fbb-515a47bf1ed9> ;
    skos:relatedMatch <http://hdl.handle.net/11459/CCR_C-4428_10017d9a-0387-0a2b-1fbb-515a47bf1ed9> .

csdtt:0078 a skos:Concept ;
    skos:altLabel "querying"@en ;
    skos:broader csdtt:0077 ;
    skos:closeMatch tadirah:searching ;
    skos:definition "request for information through a query"@en ;
    skos:inScheme csdtt: ;
    skos:prefLabel "searching"@en .

csdtt:0084 a skos:Concept ;
    rdfs:isDefinedBy <https://en.wikipedia.org/wiki/Sentiment_analysis> ;
    skos:broader tadirah:contentAnalysis,
        csdtt:0113 ;
    skos:closeMatch tadirah:sentimentAnalysis ;
    skos:definition "software to systematically identify, extract, quantify, and study affective states and subjective information"@en ;
    skos:inScheme csdtt: ;
    skos:prefLabel "sentiment analysis"@en .

csdtt:0103 a skos:Concept ;
    skos:broader tadirah:contentAnalysis,
        csdtt:0100 ;
    skos:closeMatch tadirah:topicModeling ;
    skos:definition "creation of a topic model from a text corpus"@en ;
    skos:inScheme csdtt: ;
    skos:prefLabel "topic model generation"@en .

csdtt:0105 a skos:Concept ;
    skos:definition "unclear which tool task to assign"@en ;
    skos:inScheme csdtt: ;
    skos:prefLabel "unknown"@en ;
    skos:related <http://hdl.handle.net/11459/CCR_C-2591_f769d93b-c007-d2c9-aff2-99e9177e5764> ;
    skos:relatedMatch <http://hdl.handle.net/11459/CCR_C-2591_f769d93b-c007-d2c9-aff2-99e9177e5764> ;
    skos:topConceptOf csdtt: .

csdtt:0121 a skos:Concept ;
    skos:definition ""@en ;
    skos:exactMatch tadirah:georeferencing ;
    skos:inScheme csdtt: ;
    skos:narrower csdtt:0034 ;
    skos:prefLabel "geographic linking"@en ;
    skos:topConceptOf csdtt: .

csdtt:0123 a skos:Concept ;
    skos:definition "processing or creating interpreted data"@en ;
    skos:inScheme csdtt: ;
    skos:narrower csdtt:0038,
        csdtt:0074 ;
    skos:prefLabel "information processing"@en ;
    skos:topConceptOf csdtt: .

tadirah: a skos:ConceptScheme .

tadirah:contentAnalysis skos:narrower tadirah:informationRetrieval,
        csdtt:0057,
        csdtt:0084,
        csdtt:0103 .

csdtt:0006 a skos:Concept ;
    skos:broader tadirah:enriching ;
    skos:definition "enriching data with information"@en ;
    skos:exactMatch tadirah:annotating ;
    skos:inScheme csdtt: ;
    skos:narrower csdtt:0045 ;
    skos:prefLabel "annotation"@en ;
    skos:topConceptOf csdtt: .

csdtt:0057 a skos:Concept ;
    skos:broader tadirah:annotating,
        tadirah:contentAnalysis,
        csdtt:0058 ;
    skos:closeMatch tadirah:namedEntityRecognition ;
    skos:definition "Named-entity recognition is the process of recognizing and classifying names in a text, such as personal, location and organisation names."@en ;
    skos:inScheme csdtt: ;
    skos:prefLabel "named entity recognition"@en .

csdtt:0058 a skos:Concept ;
    skos:broader csdtt:0044,
        csdtt:0045 ;
    skos:definition "processing of names"@en ;
    skos:inScheme csdtt: ;
    skos:narrower csdtt:0057 ;
    skos:prefLabel "name processing"@en ;
    skos:related csdls:0046 .

csdtt:0070 a skos:Concept ;
    skos:broader csdtt:0044,
        csdtt:0045 ;
    skos:definition "processing at the phonetic level"@en ;
    skos:inScheme csdtt: ;
    skos:narrower csdtt:0069 ;
    skos:prefLabel "phonetic processing"@en ;
    skos:related csdls:0027 .

csdtt:0086 a skos:Concept ;
    skos:broader csdtt:0044,
        csdtt:0045 ;
    skos:definition "processing at the sociolinguistics level"@en ;
    skos:inScheme csdtt: ;
    skos:narrower csdtt:0024 ;
    skos:prefLabel "sociolinguistic processing"@en ;
    skos:related csdls:0035 .

csdtt:0096 a skos:Concept ;
    skos:broader csdtt:0044,
        csdtt:0045 ;
    skos:definition "processing at the terminology level"@en ;
    skos:inScheme csdtt: ;
    skos:narrower csdtt:0097 ;
    skos:prefLabel "terminological processing"@en ;
    skos:related csdls:0044 .

csdtt:0111 a skos:Concept ;
    rdfs:isDefinedBy <https://en.wikipedia.org/wiki/Digital_image_processing> ;
    skos:broader tadirah:capturing ;
    skos:closeMatch tadirah:imaging ;
    skos:definition "Digital image processing is the use of a digital computer to process digital images through an algorithm"@en ;
    skos:inScheme csdtt: ;
    skos:narrower csdtt:0062 ;
    skos:prefLabel "image processing"@en ;
    skos:topConceptOf csdtt: .

csdtt:0004 a skos:Concept ;
    skos:definition "analysis includes selecting, sorting, grouping and  filtering of data"@en ;
    skos:exactMatch tadirah:analyzing ;
    skos:inScheme csdtt: ;
    skos:narrower csdtt:0011,
        csdtt:0032,
        csdtt:0044 ;
    skos:prefLabel "analysis"@en ;
    skos:topConceptOf csdtt: .

csdtt:0095 a skos:Concept ;
    skos:broader csdtt:0044,
        csdtt:0045 ;
    skos:definition "processing at the  syntax level"@en ;
    skos:inScheme csdtt: ;
    skos:narrower csdtt:0066,
        csdtt:0085 ;
    skos:prefLabel "syntactic processing"@en ;
    skos:related csdls:0038 .

csdtt:0114 a skos:Concept ;
    rdfs:seeAlso <https://en.wikipedia.org/wiki/Lexicon> ;
    skos:definition "a set of entries of a linguistic unit (morpheme, word, multiword expression, etc.) and its properties"@en ;
    skos:inScheme csdtt: ;
    skos:narrower csdtt:0027,
        csdtt:0041,
        csdtt:0042,
        csdtt:0043 ;
    skos:prefLabel "lexicon processing"@en ;
    skos:topConceptOf csdtt: .

csdtt:0020 a skos:Concept ;
    skos:definition "processing a corpus"@en ;
    skos:inScheme csdtt: ;
    skos:narrower tadirah:concordance,
        csdtt:0018,
        csdtt:0022,
        csdtt:0033,
        csdtt:0037 ;
    skos:prefLabel "corpus processing"@en ;
    skos:topConceptOf csdtt: .

csdtt:0028 a skos:Concept ;
    skos:broader csdtt:0044,
        csdtt:0045 ;
    skos:definition "level of linguistics dealing with the relations between co-occurring utterances"@en ;
    skos:inScheme csdtt: ;
    skos:narrower csdtt:0015,
        csdtt:0016,
        csdtt:0025,
        csdtt:0029 ;
    skos:prefLabel "discourse"@en .

csdtt:0052 a skos:Concept ;
    skos:broader csdtt:0044,
        csdtt:0045 ;
    skos:definition "processing at the morphosyntax level"@en ;
    skos:inScheme csdtt: ;
    skos:narrower csdtt:0051,
        csdtt:0067,
        csdtt:0068 ;
    skos:prefLabel "morphosyntactic processing"@en ;
    skos:related csdls:0020 .

csdtt:0077 a skos:Concept ;
    skos:definition "trying to find an object"@en ;
    skos:inScheme csdtt: ;
    skos:narrower csdtt:0021,
        csdtt:0042,
        csdtt:0043,
        csdtt:0073,
        csdtt:0078 ;
    skos:prefLabel "search"@en ;
    skos:topConceptOf csdtt: .

csdtt:0100 a skos:Concept ;
    skos:definition "processing of a text"@en ;
    skos:inScheme csdtt: ;
    skos:narrower csdtt:0093,
        csdtt:0098,
        csdtt:0099,
        csdtt:0103,
        csdtt:0113 ;
    skos:prefLabel "text processing"@en ;
    skos:topConceptOf csdtt: .

csdtt:0112 a skos:Concept ;
    skos:definition "software to process speech signals"@en ;
    skos:inScheme csdtt: ;
    skos:narrower csdtt:0026,
        csdtt:0087,
        csdtt:0088,
        csdtt:0089,
        csdtt:0101 ;
    skos:prefLabel "speech processing"@en ;
    skos:topConceptOf csdtt: .

csdtt:0056 a skos:Concept ;
    skos:broader csdtt:0044,
        csdtt:0045 ;
    skos:definition "processing of multiword expressions"@en ;
    skos:inScheme csdtt: ;
    skos:narrower tadirah:collocationAnalysis,
        csdtt:0014,
        csdtt:0054,
        csdtt:0055 ;
    skos:prefLabel "multiword expression processing"@en ;
    skos:related csdls:0047 .

csdtt:0081 a skos:Concept ;
    skos:broader csdtt:0044,
        csdtt:0045 ;
    skos:definition "processing at the semantics level"@en ;
    skos:inScheme csdtt: ;
    skos:narrower csdtt:0005,
        csdtt:0079,
        csdtt:0080,
        csdtt:0110 ;
    skos:prefLabel "semantic processing"@en ;
    skos:related csdls:0033 .

csdtt:0050 a skos:Concept ;
    skos:broader csdtt:0044,
        csdtt:0045 ;
    skos:definition "processing at the morphology level"@en ;
    skos:inScheme csdtt: ;
    skos:narrower csdtt:0012,
        csdtt:0040,
        csdtt:0049,
        csdtt:0091,
        csdtt:0109 ;
    skos:prefLabel "morphological processing"@en ;
    skos:related csdls:0021 .

csdtt:0066 a skos:Concept ;
    skos:broader csdtt:0095 ;
    skos:definition "assigning a syntactic structure to a natural language utterance"@en ;
    skos:inScheme csdtt: ;
    skos:narrower csdtt:0010,
        csdtt:0013,
        csdtt:0023,
        csdtt:0035,
        csdtt:0063,
        csdtt:0076,
        csdtt:0094 ;
    skos:prefLabel "parsing"@en .

csdtt:0064 a skos:Concept ;
    skos:broader csdtt:0044,
        csdtt:0045 ;
    skos:definition "processing at the orthography level"@en ;
    skos:inScheme csdtt: ;
    skos:narrower csdtt:0002,
        csdtt:0061,
        csdtt:0063,
        csdtt:0082,
        csdtt:0083,
        csdtt:0090,
        csdtt:0102 ;
    skos:prefLabel "orthographic processing"@en ;
    skos:related csdls:0024 .

csdtt:0113 a skos:Concept ;
    rdfs:seeAlso <https://en.wikipedia.org/wiki/Document_classification> ;
    skos:broader csdtt:0100 ;
    skos:definition "software to assign a text to one or more categories"@en ;
    skos:inScheme csdtt: ;
    skos:narrower csdtt:0008,
        csdtt:0039,
        csdtt:0072,
        csdtt:0075,
        csdtt:0084,
        csdtt:0092,
        csdtt:0104,
        csdtt:0119,
        csdtt:0120 ;
    skos:prefLabel "text categorization"@en .

csdtt:0044 a skos:Concept ;
    skos:broader csdtt:0004 ;
    skos:definition "analysis in terms of linguistic concepts"@en ;
    skos:inScheme csdtt: ;
    skos:narrower csdtt:0028,
        csdtt:0050,
        csdtt:0052,
        csdtt:0053,
        csdtt:0056,
        csdtt:0058,
        csdtt:0064,
        csdtt:0070,
        csdtt:0081,
        csdtt:0086,
        csdtt:0095,
        csdtt:0096 ;
    skos:prefLabel "linguistic analysis"@en .

csdtt:0045 a skos:Concept ;
    skos:broader csdtt:0006 ;
    skos:definition "annotation with linguistic properties"@en ;
    skos:inScheme csdtt: ;
    skos:narrower csdtt:0028,
        csdtt:0050,
        csdtt:0052,
        csdtt:0053,
        csdtt:0056,
        csdtt:0058,
        csdtt:0064,
        csdtt:0070,
        csdtt:0081,
        csdtt:0086,
        csdtt:0095,
        csdtt:0096 ;
    skos:prefLabel "linguistic annotation"@en .

csdtt: a skos:ConceptScheme ;
    dc:contributor "Jan Odijk, Daan Broeder, Eline Westerhout, Rogier Kraf, Erica Renkens" ;
    dc:title "CLARIN taxonomy for tools and services tasks"@en ;
    dct:created "2023-09-01"^^xsd:date ;
    dct:description "Tool tasks is a taxonomy for classifying task(s) carried out by services and tools such as we encounter these in the CLARIN domain, and/or a typical task description of the software."@en ;
    dct:language iso639-3:eng,
        iso639-3:nld ;
    dct:license <https://creativecommons.org/publicdomain/zero/1.0> ;
    dct:modified "2024-01-02"^^xsd:date ;
    dct:relation <http://hdl.handle.net/11459/CCR_C-2500_a16d939a-58e3-121d-aaa3-05237ec2d206> ;
    owl:versionInfo "1.3.0"^^xsd:string ;
    skos:hasTopConcept csdtt:0000,
        csdtt:0004,
        csdtt:0006,
        csdtt:0007,
        csdtt:0019,
        csdtt:0020,
        csdtt:0030,
        csdtt:0031,
        csdtt:0065,
        csdtt:0071,
        csdtt:0077,
        csdtt:0100,
        csdtt:0105,
        csdtt:0111,
        csdtt:0112,
        csdtt:0114,
        csdtt:0121,
        csdtt:0122,
        csdtt:0123,
        csdtt:0124,
        csdtt:0125,
        csdtt:0126,
        csdtt:0127,
        csdtt:0128 ;
    skos:prefLabel "CLARIN Services Description Tool Task taxonomy"@en .

